\begin{enumerate}
\item If $\nu$ is a signed measure, $E$ is $\nu-$null if and only if $|\nu|(E)=0$.
\begin{pf}
$(\Rightarrow)$ Since $\nu$ is a signed measure, we can write $X= P \cup N$. Assume $E$ is $\nu-$null. Then, $\nu(E)=0$. Then, $\nu(E \cap P)=0$ and $\nu(E \cap N)=0$. Thus, $\nu^+(E)=0$ and $\nu^-(E)=0$ and so $|\nu|(E)= \nu^+(E)+\nu^-(E)=0$. Hence, $|\nu|(E)=0$.
\\
$(\Leftarrow)$ Assume $|\nu|(E)=0$. Then, $\nu^+(E) + \nu^-(E)=0$. Since $\nu^+, \nu^-$ are positive, we have $\nu^+(E)=0$ and $\nu^-(E)=0$. Then, for any subset $F$ in $E$ so $F \cap P \subset E$ and $F \cap N \subset E$ so $\nu^+(F \cap P)=0$ and $\nu^-(F \cap N)=0$. Hence,
\[
\nu(F)=\nu^+(F \cap P) - \nu^-(F \cap N) = 0 - 0 = 0.
\]

\end{pf}

\item If $\nu$ and $\sigma$ are signed measures then $\nu \perp \sigma$ if and only if $\nu \perp |\sigma|$ if and only if $\nu^+ \perp \sigma$ and $\nu^- \perp \sigma$.
\\
\[
\textbf{Denote a: } \nu \perp \sigma, \textbf{   b: } \nu \perp |\sigma|, \textbf{   c: } \nu^+ \perp \sigma, \nu^- \perp \sigma
\]
\textbf{(a $\Rightarrow$ b) } Assume $\nu \perp \sigma$. Then, there exist $E, F$ such that $X = E \cup F$, $E$ is $\sigma$-null, and $F$ is $\nu$-null. Then, since $E$ is $\sigma$-null for any $A \subseteq E$, $\sigma(A) = \sigma^+(A) - \sigma^-(A)=0$. Thus, $\sigma^+(A)=0$ and $\sigma^-(A)=0$. Hence for any $A \subseteq E$, $|\sigma|(A) = \sigma^+(A)+\sigma^-(A) = 0$. Thus, $E$ is $|\sigma|$-null. So there exist $E, F$ such that $X = E \cup F$, $E$ is $|\sigma|$-null, and $F$ is $\nu$-null. Hence $\nu \perp |\sigma|$.
\\
\textbf{ (a $\Rightarrow$ c) } 
Assume $\nu \perp \sigma$. Then, there exist $E, F$ such that $X = E \cup F$, $E$ is $\sigma$-null, and $F$ is $\nu$-null. Since $F$ is $\nu$-null, for any $A \subseteq F$, $\nu(A)=0$. Let $F= P \cup N$ then $P \subseteq F, N \subseteq F$, so $\nu(P)=0=\nu(N)$. Hence, for any $A \subseteq F$,
\[
\nu^+(A) = \nu(A \cap P) = 0, \text{ and } \nu^-(A) = \nu(A \cap N) = 0.
\]
Thus, $F$ is $\nu^+$-null and $F$ is $\nu^-$-null. So, $E, F$ satisfy the conditions for $\nu^+ \perp \sigma$ and $\nu^- \perp \sigma$.
\\
\textbf{(b $\Rightarrow$ a) } Assume $\nu \perp |\sigma|$. Then, there exist $E, F$ such that $X = E \cup F$, $E$ is $\nu$-null, and $F$ is $|\sigma|$-null. The, since $F$ is $|\sigma|$-null, for any $A \subseteq F$, $|\sigma|(A)=0$ and so $\sigma^+(A) + \sigma^-(A)=0$. $\sigma^+, \sigma^-$ are finite so $\sigma^+(A) + \sigma^-(A)=0$ implies $\sigma^+(A)=0=\sigma^-(A)$. Thus, $\sigma(A) = \sigma^+(A) - \sigma^-(A) = 0 $ so $F$ is $\sigma$-null. Hence, $\nu \perp \sigma$.
\\
\textbf{(c $\Rightarrow$ a) } \\
Assume $\nu^+ \perp \sigma, \nu^- \perp \sigma$. Then, there exist $E_1, F_1$ such that $X = E_1 \cup F_1$, $E_1$ is $\sigma$-null, and $F_1$ is $\nu^+$-null and there exists $E_2, F_2$ such that $X = E_2 \cup F_2$, $E_2$ is $\sigma$-null, and $F_2$ is $\nu^+$-null. First, we will show $E = E_1 \cup E_2 $ is $\sigma$-null. Consider any $A \subseteq E_1 \cup E_2$. Then, $A = A \cap (E_1 \cup E_2)= (A \cap E_1) \cup (A \cap E_2)$. Since $E_1, E_2$ are $\sigma$-null, $\sigma(A)= \sigma(A \cap E_1) + \sigma (A \cap E_2)=0$. Thus, $E_1 \cup E_2$ is $\sigma$-null.
Next, we will show $F = F_1 \cap F_2$ is $\nu$-null. Consider any $A \subseteq F_1 \cap F_2$. Then, $A \subseteq F_1$ and $A \subseteq F_2$ so $\nu^+(A)=0$ and $\nu^-(A)=0$. Thus, $\nu(A)=\nu^+(A)-\nu^-(A)=0$. So, $F$ is $\nu$-null.
Finally, notice
\[
(E_1 \cup E_2)^c = F_1 \cap F_2. \text{ So, } (E_1 \cup E_2) \cup (F_1 \cap F_2) = X \text{ and } (E_1 \cup E_2) \cap (F_1 \cap F_2) = \O
\]
Hence, $\nu \perp \sigma$.
\item Suppose $\nu(E) = \int_E f d \mu$ where $\mu$ is a positive measure and $f$ is a $\mu-$integrable function (not necessarily positive). Describe the Hahn decompositions of $\nu$ and the positive, negative, and total variations of $\nu$ in terms of $f$ and $\mu$. 	
\\
Let $P= \{x : f(x) > 0\}$ and $N = \{ x: f(x) \leq 0 \}$. Note $P=f^{-1}(0, \infty)$ and $N = f^{-1}((-\infty, 0])$. Since $f$ is $\mu$ measurable, $P$ and $N$ are measurable.  Also,

\[
\nu^+(E)= \nu(E \cap P)= \int_{E \cap P}f d \mu \text{ and } \nu^-(E) = \nu(E \cap N) = - \int_{E \cap N} f d \mu.
\]
\[
 \text{ Hence, } |\nu|(E) = \int_{E \cap P}f d \mu- \int_{E \cap N} f d \mu.
\]
\end{enumerate}
