(1) Suppose that $\mu$ and $\nu$ are $\sigma$-finite measures on $(X, \M)$ with $\nu \ll \mu$, and let $\lambda = \mu + \nu$. If $f = \frac{d \nu}{d \lambda}$ then prove that $0 \leq f < 1$ $\mu$-a.e. and $\frac{d \nu}{d \mu}=\frac{f}{1-f}$.\\
\begin{proof}
	Suppose that $\mu$ and $\nu$ are $\sigma$-finite measures on $(X, \M)$ with $\nu \ll \mu$, and let $\lambda = \mu + \nu$. First, we will show $\nu \ll \lambda , \mu \ll \lambda , \lambda \ll \mu$. Suppose $\lambda(E) = 0$. Then, $\lambda(E)= (\mu + \nu)(E) = \mu(E) + \nu(E) = 0 $. Since $\mu, \nu$ are positive, finite measures this implies $\mu(E) = \nu(E) = 0$. Thus, $\mu \ll \lambda$ and $\nu \ll \lambda$. 
	 Let \[
f = \frac{d \nu}{d \lambda }, \quad h = \frac{d \nu}{d \mu}, \quad j = \frac{d \lambda}{d \mu}, \quad g =\frac{d \mu}{d \lambda}.
	\] 
	\begin{eqnarray*}
\text{ Then, } 1 = g + f & \text{ and } & 1 = g + gh \\
	\frac{1}{g} & = & 1 + h \\
	h & = & \frac{1}{g} - 1 \\
	h & = & \frac{1-g}{g}\\
	& = & \frac{f}{1-g}
	\end{eqnarray*}
\[
\text{Hence, } \frac{d \nu}{d \mu}=\frac{f}{1-f}.
\]
To show $0 \leq f < 1$ $\mu$-a.e., first note that $f + g = 1$. Suppose $f \geq 1$ on some $A$ such that $\nu(A)>0$. Then, $\lambda(A)>0$ and
\[
 \nu(A) = \int_A f d \lambda < \int_A 0 d \lambda = 0, \text{ which is a contradiction. }
\]
Therefore, $f>0$. Next, suppose $f>1$ on some $A$ such that $\mu(A)>0$. Then, $\lambda(A)>0$ and 
\[
\nu(A) = \int_A f d \lambda \geq \int_A 1 d \lambda = \lambda(A) = \mu(A) + \nu(A)> \nu(A) \text{ which is a contradiction.}
\]
Hence, $0< f \leq 1$. 
\end{proof}
