\begin{enumerate}
\item Suppose that $\mu_1$ and $\nu_1$ are $\sigma$-finite measures on $(X_1, \M_1)$ with $\nu_1 \ll \mu_1$. Similarly, assume that $\mu_2, \nu_2$ are $\sigma$-finite measures on $(X_2, \M_2)$ with $\nu_2 \ll \mu_2$. Prove that $\nu_1 \times \nu_2 \ll \mu_1 \times \mu_2$.
\begin{pf}
Suppose that $\mu_1$ and $\nu_1$ are $\sigma$-finite measures on $(X_1, \M_1)$ with $\nu_1 \ll \mu_1$. Similarly, assume that $\mu_2, \nu_2$ are $\sigma$-finite measures on $(X_2, \M_2)$ with $\nu_2 \ll \mu_2$. Assume $\mu_1 \times \mu_2 (E) = 0$. 
\begin{eqnarray*}
\text{Then, } 0=\mu_1 \times \mu_2 (E) & = & \int \chi_E d (\mu_1 \times \mu_2) \\
 & = & \int \int (\chi_E)_{x_2} d \mu_1 d \mu_2 \\
 & = & \int \mu_1\left( (\chi_E)_{x_2} \right) d \mu_2
\end{eqnarray*}
By Fubini, if $\int \mu_1 \left( (\chi_E)_{x_2} \right) d \mu_2=0$, $\int \mu_2\left( (\chi_E)^{x_1} \right) d \mu_1=0$ which imply $\mu_1\left( (\chi_E)_{x_2} \right)=0$ and $\mu_2\left( (\chi_E)^{x_1} \right)=0$. Then, by assumption, $\nu_1\left( (\chi_E)_{x_2} \right)=0$ and $\nu_2\left( (\chi_E)^{x_1} \right)=0$. Thus,
\begin{eqnarray*}
\nu_1 \times \nu_2 (E) &=& \int \chi_E d \nu_1 \times \nu_2\\
&=& \int \int (\chi_E)^{x_1} d \nu_2 d \nu_1 \\
&=& \int \nu_2\left( (\chi_E)^{x_1} \right)  d \nu_1 	\\
&=& \int 0  d \nu_1 \\
& = & 0
\end{eqnarray*}
Thus, $\nu_1 \times \nu_2 \ll \mu_1 \times \mu_2$. 
\end{pf}
 \[
\text{ Given the same conditions as in (1), prove that }\frac{d(\nu_1 \times \nu_2)}{d(\mu_1 \times \mu_2)}= \frac{d \nu_1}{d \mu_1}.  
\] 
\begin{pf}
	Suppose $E_1 \in \M_1$, $E_2 \in \M_2$, $x_1 \in X_1, x_2 \in X_2$. Then, we have
	\[
	\frac{d \nu_1}{d \mu_1} = f_1(x_1), \nu_1(E_1)= \int_{E_1} f_1 (x_1) d \mu_1 \quad \text{ and } \quad  \frac{d \nu_2}{d \mu_2} = f_2(x_2), \nu_2(E_2)= \int_{E_2} f_2 (x_2) d \mu_2.
	\]
\begin{eqnarray*}
	\text{ Then, } (\nu_1 \times \nu_2)(E_1 \times E_2) &=& \nu_1(E_1) \nu_2(E_2)\\
	& = & \int_{E_1} f_1 (x_1) d \mu_1 \int_{E_2} f_2 (x_2) d \mu_2 \\
	& = & \int_{E_2} \int_{E_1} f_1 (x_1) f_2 (x_2) d \mu_1   d \mu_2 \\
	& = & \int_{E_1 \times E_2} f_1 f_2 d (\mu_1 \times \mu_2)
\end{eqnarray*}
Since $f_1f_2$ must be unique and $(\nu_1 \times \nu_2)(E_1 \times E_2) = \int_{E_1 \times E_2} f_1 f_2 d (\mu_1 \times \mu_2)$, 
\[
\frac{d(\nu_1 \times \nu_2)}{d(\mu_1 \times \mu_2)}= f_1 f_2 = \frac{d \nu_1}{d \mu_1}   \frac{d \nu_2}{d \mu_2}
\]
\end{pf}
\item Let $X= [0,1]$, $\M = \B_{[0,1]}$, $m=$ Lebesgue measure and $\mu=$ counting measure. Prove that $m \ll \mu$ but there is no $f$ such that $dm = f d \mu$.
\begin{pf}
	For $E \in \M$ suppose $\mu(E)=0$. Then, $E = \O$ and so $m(E)=0$. Thus, $m \ll \mu$. Next, suppose there is an $f$ such that $dm = f d \mu$. Let $a \in [0, 1]$ and note $m(\{ a \})=0$ and 
	\[
	m(\{a\}) = \int_{\{a\}} f d \mu = f(a) \mu (\{ a \}) = f(a). \qquad \text{ Hence, } f(a) = 0 \quad \forall \ a \in [0,1].
	\]
	Also, notice $m([0,1])=1$ but 
	\[
	m([0,1]) = \int_{[0,1]}f d \mu = \int 0 d \mu = 0 \mu([0,1]) = 0.
	\]
	Thus, there is no $f$ such that $dm = f d \mu$.
\end{pf}
\end{enumerate}
