\begin{enumerate}
\item Prove that $(a,\infty)$ is $m^*$-measurable for any $a$.\begin{pf}
We will show for any set $E$, $m^{*}(E)=m^{*}(E \cap (a, \infty))+ m^{*}(E \cap (-\infty, a])$. 
If $m^{*}(E)= \infty$, since $m^{*}((a, \infty))=m^{*}((-\infty, a])= \infty$, the above equality will hold, so assume $m^{*}(E) < \infty$. Notice for any set $E$, $E=(E \cap (a, \infty)) \cup (E \cap (-\infty, a])$ so by subadditivity of $m^{*}$, we have
 \[
 m^{*}(E)\leq m*(E \cap (a, \infty)) + m^{*}(E \cap (-\infty, a]). \]
 Thus, we must show $m^{*}(E)\geq m^{*}(E \cap (a, \infty)) + m^{*}(E \cap (-\infty, a])$:\\
 Let $\varepsilon >0$. By definition of $m^{*}$, there exists \[
 \bigcup_{i=1}^\infty(a_i, b_i) \text{ with } E \subset \bigcup_{i=1}^\infty(a_i, b_i) \text{ and } \sum_{i=1}^\infty(b_i-a_i) \leq m^{*}(E) + \varepsilon.
 \]
Define $(a_i, b_i)'=(a, \infty) \cap (a_i, b_i)$ and $(a_i, b_i)''= (-\infty, a] \cap (a_i, b_i)$. 
Notice 
$
\left( (a, \infty) \cap (a_i, b_i) \right) \cup \left( (-\infty, a] \cap (a_i, b_i) \right) = (a_i, b_i). 
$
Then, $m^{*}(a_i, b_i) = b_i - a_i=m^{*}((a_i,b_i)')+m^{*}((a_i, b_i)'')$.\\
	Since $E \subset (a_i, b_i)$ for any $i$ and $E \cap (a, \infty) \subset (a_i, b_i) \cap (a,\infty) \subset \bigcup_{i=1}^\infty(a_i, b_i)'$. So, by monotonicity and subadditivity of $m^{*}$, 
	\[
	m^{*}(E \cap (a, \infty)) \leq  m^{*}\left(\bigcup_{i=1}^\infty(a_i, b_i)'\right) \leq \sum_{i=1}^\infty m^{*}((a_i, b_i)').
	\] Similarly, since $E \subset (a_i, b_i)$ for any $i$ and $E \cap (- \infty, a] \subset (a_i, b_i) \cap (- \infty, a] \subset \bigcup_{i=1}^\infty(a_i, b_i)''$. So, by monotonicity and subadditivity of $m^{*}$, 
	\[
	\begin{multlined}
	\qquad \qquad \qquad \qquad m^{*}(E \cap (- \infty, a]) \leq  m^{*}\left(\bigcup_{i=1}^\infty(a_i, b_i)''\right) \leq \sum_{i=1}^\infty m^{*}((a_i, b_i)''). \text{ Thus, } \\
	m^{*}(E \cap (a, \infty)) + m^{*}(E \cap (- \infty, a]) \leq \sum_{i=1}^\infty m^{*}((a_i, b_i)') +\sum_{i=1}^\infty m^{*}((a_i, b_i)'')=\sum_{i=1}^\infty \left( m^{*}((a_i, b_i)') + m^{*}((a_i, b_i)'') \right)\\
	=\sum_{i=1}^\infty (b_i - a_i) \leq m^{*}(E) + \varepsilon. \text{ Hence, } m^{*}(E)\geq m^{*}(E \cap (a, \infty)) + m^{*}(E \cap (- \infty, a]). \qquad \qquad \qquad
	\end{multlined}
	\]
Thus, $(a, \infty)$ is $m^{*}$-measurable. 
\end{pf}
\item Prove that any Borel set is $m^*$-measurable. 
	\begin{pf}
In (1) we showed that $(a, \infty)$ is $m^*$-measurable. From exercise 1 on August 31, we know that $\M(\lbrace (a, \infty): a \in \R \rbrace)= \B_\R$. Since the collection of $m^{*}$-measurable sets is a $\sa$, any Borel set is $m^*$-measurable. 
\end{pf}

\item Prove that for any set $E$ and any $\varepsilon > 0$ there is an open set $A$ with $E \subseteq A$ such that $m^*(A)\leq m^*(E)+\varepsilon$. 
\begin{pf}
Consider any set $E$. Then \[
m^{*}(E)=\inf \left\lbrace \sum_{i=1}^\infty (b_i - a_i) \colon \ E \subseteq \bigcup_{i=1}^\infty (a_i, b_i) \right\rbrace.
\]
Then, for any $\varepsilon>0$ there exists some $\lbrace (a_i, b_i)\rbrace _{i=1}^\infty$ such that $m^{*}(E) + \varepsilon \geq \sum_{i = 1}^\infty (b_i-a_i)$ with $E \subseteq \bigcup_{i=1}^\infty (a_i, b_i)$. Let $A=\bigcup_{i=1}^\infty (a_i, b_i)$. Note $A$ is an open set. Then, $m^{*}(A)\leq \sum_{i=1}^\infty (b_i-a_i)$. Hence, $m^{*}(E) + \varepsilon \geq m^{*}(A)$.
\end{pf}

\item Let $E$ be a given set. Prove the following are equivalent.
(a) $E$ is $m^*$-measurable. (b) Given $\varepsilon>0$ there is an open set $O \supset E$ such that $m^*(O\backslash E)<\varepsilon$. (c) Given $\varepsilon>0$ there is an closed set $K \subset E$ such that $m^*(E\backslash K)<\varepsilon$. (d) There is a $G_{\delta}$ set $G$ with $E \subseteq G$ and $m^*(G \backslash E)=0$\ . (e) There is a $F_{\sigma}$ set $F$ with $F \subseteq E$ and $m^*(E \backslash F)=0$.
\begin{pf}[\textbf{(a $\Rightarrow$ b)}]
Assume $E$ is $m^{*}$-measurable. Suppose $m^{*}(E)<\infty$. Then, since \\$m^{*}(E)=\inf \left\lbrace \sum_{i=1}^\infty (b_i - a_i) \colon \ E \subseteq \bigcup_{i=1}^\infty (a_i, b_i) \right\rbrace$, given $\varepsilon>0$, there exists some cover of $E, \bigcup_{i=1}^\infty (a_i, b_i)$ such that $\sum_{i=1}^\infty (b_i - a_i) < m^{*}(E) + \varepsilon$. Let $O=\bigcup_{i=1}^\infty (a_i, b_i)$. Then, $O$ is open and by subadditivity of $m^{*}$, $m^{*}(O)=m^{*}(\bigcup_{i=1}^\infty (a_i, b_i)) \leq \sum_{i=1}^\infty (b_i-a_i)$. Thus, $m^{*}(O) < m^{*}(E) + \varepsilon$. Since $m^{*}(E)<\infty$, we can subtract $m^{*}(E)$ from both sides of the previous inequality to obtain,  $m^{*}(O) - m^{*}(E) < \varepsilon$. Equivalently, $m^{*}(O \backslash E) < \varepsilon$.\\
Now, suppose $m^{*}(E)=\infty$. Then, $E=E\cap \R$ and $\R=\bigcup_{i=1}^{\infty}[-i, i]$ so $E=\bigcup_{i=1}^{\infty}[-i, i] \ \cap \ E$. For all $i$, let $E_i=[-i, i] \ \cap \ E$. Then, since $m^{*}([-i, i])=2i$, the measure of $E_i$ must be finite. From the previous paragraph, if $E_i < \infty$ there exists some open set $O_i$ with $O_i \supset E_i$ such that 
\[
m^{*}(O_i \backslash E_i) < \frac{\varepsilon}{2^i}.
\] 
Let $O=\bigcup_{i=1}^\infty(O_i)$. Then, $O$ is open and since $O_i \supset E_i$, $\bigcup_{i=1}^\infty(O_i)\supset \bigcup_{i=1}^\infty(E_i)$. Therfore, $O\supset E$ and $O \backslash E=\bigcup_{i=1}^\infty(O_i\backslash E_i)$. (I think I need to prove the previous statement) Thus, \[
m^{*}(O \backslash E)=m^{*}\left(\bigcup_{i=1}^\infty(O_i\backslash E_i)\right)\leq \sum_{i=1}^\infty m^{*}(O_i \backslash E_i)< \sum_{i=1}^\infty\frac{\varepsilon}{2^i}=\varepsilon. 
\]
\end{pf}
\begin{pf}[\textbf{(b $\Rightarrow$ c)}]
Assume given $\varepsilon>0$ there is an open set $O \supset E$ such that $m^*(O\backslash E)<\varepsilon$. Then for $E^c$, given $\varepsilon>0$ there is an open set $O \supset E^c$ such that $m^*(O\backslash E^c)<\varepsilon$. Let $K=O^c$. Then, $K$ is closed. If $O \supset E^c$, $O^c \subset E^{c^c}$ which implies $K \subset E$. Also $O \cap E^c= O \cap E= E\backslash O^c = E\backslash K$, so $m^*(O\backslash E^c)<\varepsilon$ implies $m^{*}(E \backslash K)<\varepsilon$. 
\end{pf}

\begin{pf}[\textbf{(b $\Rightarrow$ d)}]
	Assume given $\varepsilon>0$ there is an open set $O \supset E$ such that $m^*(O\backslash E)<\varepsilon$. Pick $\varepsilon=\frac{1}{i}$. Then, there must exist some open set $O_i$ such that $m^{*}(O_i \backslash E) < \frac{1}{i}$ for any $i$. Let $G = \cap_{i=1}^\infty O_i$. Then, $G$ is the countable intersection of open sets, so $G$ is a $G_\delta$ set. $E \subset O_i$ for all $i$ implies $E \subset \cap_{i=1}^\infty O_i$ so $E \subset G$. Also notice $G \backslash E = (\cap_{i=1}^\infty O_i)\backslash E=(\cap_{i=1}^\infty O_i)\cap E^c=\cap_{i=1}^\infty (O_i\cap E^c)= \cap_{i=1}^\infty (O_i\backslash E)$; thus $G \backslash E = \cap_{i=1}^\infty (O_i\backslash E)$. Since $\cap_{i=1}^\infty (O_i\backslash E)\subset O_i \backslash E$ for any $i$, monotonicity of $m^{*}$ implies $m^{*}(\cap_{i=1}^\infty (O_i\backslash E)) \leq m^{*}(O_i \backslash E)$. Hence $m^{*}(G \backslash E) = m^{*}(\cap_{i=1}^\infty (O_i\backslash E))\leq  m^{*}(O_i \backslash E) \leq \frac{1}{i}$ for any $i \geq 1$. Thus,  $m^{*}(G \backslash E) = 0$. 
\end{pf}

\begin{pf}[\textbf{(d $\Rightarrow$ a)}]
Let $E$ be any subset of $\R$. Assume there is a $G_{\delta}$ set $G$ with $E \subseteq G$ and $m^*(G \backslash E)=0$. From exercise 2 on September 18, we know all Borel sets are $m^{*}$-measurable, so $G$ is $m^{*}$-measurable. Also, since $m^*(G \backslash E)=0$, by exercise 2 on September 21, we know $G \backslash E$ is $m^{*}$-measurable. Because the collection of $m^{*}$-measurable sets forms a $\sa$ we know if $G \backslash E $ is $  m^{*}$-measurable then $(G \backslash E)^c$ is $  m^{*}$-measurable and also $G \cap (G \backslash E)^c$ is $m^{*}$-measurable. Notice 
\[
G \cap (G \backslash E)^c = G \cap (G \cap E^c)^c = G \cap (G^c \cup E) = (G \cap G^c) \cup (G \cap E) = \o \cup (G \cap E) = G \cap E.
\]
Since $E \subseteq G$, $G \cap E=E$. Therefore, $E$ is $m^{*}$-measurable.
\end{pf}

\begin{pf}[\textbf{(c $\Rightarrow$ e)}]
	Assume given any $\varepsilon>0$ there is an closed set $K \subset E$ such that $m^*(E\backslash K)<\varepsilon$. Pick $\varepsilon=\frac{1}{i}$. Then, there must exist some closed set $K_i$ such that $m^{*}(E \backslash K_i) < \frac{1}{i}$ for any $i$. Let $F = \cup_{i=1}^\infty K_i$. Then, $F$ is the countable union of closed sets, so $F$ is a $F_\sigma$ set. $K_i \subset E$ for all $i$ implies $\cup_{i=1}^\infty K_i \subset E$ so $F \subset E$. Also notice $E \backslash F = E\backslash \cup_{i=1}^\infty K_i =E \cap (\cup_{i=1}^\infty K_i)^c= E \cap (\cap_{i=1}^\infty K_i^c)= \cap_{i=1}^\infty (E \cap K_i^c) = \cap_{i=1}^\infty (E \backslash K_i) $; thus $E \backslash F = \cap_{i=1}^\infty (E \backslash K_i)$. Since $\cap_{i=1}^\infty (E \backslash K_i) \subset E \backslash K_i$ for any $i$, monotonicity of $m^{*}$ implies $m^{*}(\cap_{i=1}^\infty (E \backslash K_i)) \leq m^{*}(E \backslash K_i)$. Hence $m^{*}(E \backslash F) = m^{*}(\cap_{i=1}^\infty (E\backslash K_i))\leq  m^{*}(E \backslash K_i) \leq \frac{1}{i}$ for any $i \geq 1$. Thus,  $m^*(E \backslash F)=0$.
\end{pf}
\begin{pf}[\textbf{(e $\Rightarrow$ a)}]
Let $E$ be any subset of $\R$. Assume there is a $F_{\sigma}$ set $F$ with $F \subseteq E$ and $m^*(E \backslash F)=0$. From exercise 2 on September 18, we know all Borel sets are $m^{*}$-measurable, so $F$ is $m^{*}$-measurable. Also, since $m^*(E \backslash F)=0$, by exercise 2 on September 21, we know $E \backslash F$ is $m^{*}$-measurable. Because the collection of $m^{*}$-measurable sets forms a $\sa$ we know if $E \backslash F $ is $  m^{*}$-measurable then $(E \backslash F)^c$ is $  m^{*}$-measurable and also $F^c$ is $m^{*}$-measurable and $F^c \cap (E \backslash F)^c$ is $m^{*}$-measurable. Notice 
\[
F^c \cap (E \backslash F)^c= F^c \cap (E^c \cup F) = (F^c \cap E^c) \cup (F^c \cap F)= (F^c \cap E^c) \cup \o = F^c \cap E^c .
\]
Since $F \subseteq E$, $F^c \cap E^c = E^c$. Therefore, $E^c$ is $m^{*}$-measurable. Since the collection of $m^{*}$-measurable sets forms a $\sa$, $E$ is $m^{*}$-measurable. 
\end{pf}

\end{enumerate}